---
layout: post
title: "Examples 5 and 6"
categories: maths logic
---

Examples 5 and 6 from Kleene's IM (1952) page 149

{% include mathjax.html %}


# Intro

In Kleene's IM page 149 the reader is asked to supply the details for the
following two examples.

Example 5. Given $$A(x) \vdash B$$ and $$A(x) \vdash \lnot B$$ with x held
constant, then $$\vdash \lnot A(x)$$ and $$\vdash \forall x \lnot A(x)$$.

Example 6. Given $$A(x) \vdash^x B$$ and $$A(x) \vdash^x \lnot B$$ with x not
necessarily held constant, then $$\vdash \lnot \forall x A(x)$$.

# Recap of the relevant rules

To recap, here are some rules that we're going to use, listed by Kleene as
Theorem 2, [which are natural deduction-like rules][im-postulates]:

<table>
<tr>
  <th>Implication introduction<br/>Deduction theorem</th>
  <td>If \(\Gamma, A \vdash B\)<br/>then \(\Gamma \vdash A \to B\)</td>
</tr>
<tr>
  <th>Negation introduction<br/>Reductio ad absurdum</th>
  <td>If \(\Gamma, A \vdash B\) and \(\Gamma, A \vdash \lnot B\)<br/>then
  \(\Gamma \vdash \lnot A\)</td>
</tr>
<tr>
  <th>Negation elimination<br/>Discharge of double negation</th>
  <td>\(\lnot \lnot A \vdash A\)</td>
</tr>
<tr>
  <th>Generality introduction</th>
  <td>\(A(x) \vdash^x \forall x A(x)\)</td>
</tr>
<tr>
  <th>Generality elimination</th>
  <td>\(\forall x A(x) \vdash A(t)\)</td>
</tr>
</table>

The issue is that the deduction theorem comes with a restriction: that in the
subsidiary deduction, $$\Gamma, A \vdash B$$, the free variables are [held
constant][deduction-dependent] for the assumption formula to be discharged,
$$A$$ in this case.

This comes with two consequences.

First, similar restrictions apply to other rules that involve subsidiary
deductions, in particular to the negation introduction rule above for the $$A$$
in the two subsidiary deductions.

Second, he introduces a superscript notation $$\vdash^x$$ to keep track of
deductions where postulate Rule 9 or 12 were applied with respect to $$x$$. For
example that is the case for the generality introduction. The notation is
ambiguous, e.g. it does not specify to which assumption it applies, but it's
clear from context, e.g. in the generality introduction there is only one
assumption to which it applies.

The superscript can be discharged despite the application of Rule 9 or 12 with
respect to $$x$$ in circumstances like:
- the assumption does not contain $$x$$ free
- we end up with no assumption

Kleene uses the superscript discharge in IM several times e.g.:
- on the same page 149, in the two circumstances above for Example 2 at step 2
  and Example 3 at step 3.
- on page 147 for the proofs of $$^*65$$ case 2 and $$^*68$$ case 2.

Note that the generality elimination has no restrictions: no superscript and it
has not subsidiary deduction. It does require however that the term $$t$$ is
free for $$x$$ in $$A(x)$$.

By combining generality introduction and generality elimination we get the
substitution rule that $$A(x) \vdash^x A(t)$$, requiring that the term $$t$$ is
free for $$x$$ in $$A(x)$$ (like in the generality elimination) and with the
superscript indicating that Rule 9 was used to deduce $$A(t)$$ dependent on the
assumption $$A(x)$$ (like in the generality introduction).


# For Example 5

1. $$A(x) \vdash B$$ - given
2. $$A(x) \vdash \lnot B$$ - also given
3. $$\vdash \lnot A(x)$$ - by negation introduction (on 1 and 2)
4. $$\lnot A(x) \vdash^x \forall x \lnot A(x)$$ - by generality introduction
5. $$\vdash \lnot A(x) \vdash^x \forall x \lnot A(x)$$ - from 3 and 4 we have
this chain
6. $$\vdash \forall x \lnot A(x)$$ - from 5 (notice the discharge of
superscript, i.e. $$\vdash$$ instead of $$\vdash^x$$, there are no assumptions
on the left side)


# For Example 6:

1. $$A(x) \vdash^x B$$ - given
2. $$\forall x A(x) \vdash A(x)$$ - by generality elimination
3. $$\forall x A(x) \vdash A(x) \vdash^x B$$ - from 1 and 2 we have this chain
4. $$\forall x A(x) \vdash B$$ - from 3 (notice the discharge of superscript,
because $$x$$ does not occur free in $$\forall x A(x)$$, all free occurrences
of $$x$$ in $$A(x)$$ are bound by $$\forall x$$)
5. $$\forall x A(x) \vdash \lnot B$$ similarly from the other given deduction
6. $$\lnot \vdash \forall x A(x)$$ - by negation introduction (on 4 and 5)


# Meaning

Following the ideas from the Example 3 and 4 on the same page we have: $$b \ne
0 \vdash^b 0 \ne 0$$, by the substitution rule following Theorem 2 where we
substituted $$b$$ with a term $$0$$, which is free for the variable $$b$$ in
the formula $$b \ne 0$$. The superscript indicates that $$b$$ was varied: that
we applied Rule 9 on the free variable $$b$$ in $$b \ne 0$$ and the resulting
formula is dependent on the assumption.

Also note that $$\ne$$ is an abbreviation for negating the equality formula.

The formula $$b \ne 0$$ has the conditional interpretation in Kleene: "some
natural number b is not zero". It is not a theorem.

On the other side we have $$\vdash 0 = 0$$, therefore by adding as a dummy
assumption we have $$b \ne 0 \vdash 0 = 0$$.

We can apply Example 5 and 6 by taking:
- $$x$$ to be $$b$$
- $$A(x)$$ to be $$b \ne 0$$
- $$B$$ to be $$0 = 0$$

If we apply Example 6 we get $$\vdash \lnot \forall x b \ne 0$$ which we can
interpret like "it's not true that all natural numbers are not zero".

It would be incorrect to apply Example 5, because we would incorrectly apply
the negation introduction at step 2 in the proof for Example 5. We would then
incorrectly derive (also using the discharge of the double negation) that:
$$\vdash b = 0$$ and $$\vdash \forall b (b = 0)$$. In Kleene's system theorems
have the generality interpretation and would read: "all natural numbers are
zero".


[im-postulates]:           {% post_url 2021-04-04-im-postulates %}
[deduction-dependent]:     {% post_url 2021-09-24-deduction-dependent %}
